current status

src/FcEtt/ett_ott.v
@@ -71,15 +71,17 @@ Inductive sort : Set :=  (*r binding classifier *)
  | Tm (A:tm) (R:role)
  | Co (phi:constraint).
 
+Definition context : Set := list ( atom * sort ).
+
 Inductive sig_sort : Set :=  (*r signature classifier *)
  | Cs (A:tm)
  | Ax (a:tm) (A:tm) (R:role).
 
-Definition context : Set := list ( atom * sort ).
+Definition available_props : Type := atoms.
 
 Definition sig : Set := list (atom * sig_sort).
 
-Definition available_props : Type := atoms.
+Definition role_context : Set := list ( atom * role ).
 
 (* EXPERIMENTAL *)
 (** auxiliary functions on the new list types *)
@@ -217,22 +219,16 @@ with open_constraint_wrt_tm_rec (k:nat) (a5:tm) (phi5:constraint) : constraint :
   | (Eq a b A R) => Eq (open_tm_wrt_tm_rec k a5 a) (open_tm_wrt_tm_rec k a5 b) (open_tm_wrt_tm_rec k a5 A) R
 end.
 
-Definition open_sort_wrt_co_rec (k:nat) (g5:co) (sort5:sort) : sort :=
-  match sort5 with
-  | (Tm A R) => Tm (open_tm_wrt_co_rec k g5 A) R
-  | (Co phi) => Co (open_constraint_wrt_co_rec k g5 phi)
-end.
-
 Definition open_sig_sort_wrt_co_rec (k:nat) (g5:co) (sig_sort5:sig_sort) : sig_sort :=
   match sig_sort5 with
   | (Cs A) => Cs (open_tm_wrt_co_rec k g5 A)
   | (Ax a A R) => Ax (open_tm_wrt_co_rec k g5 a) (open_tm_wrt_co_rec k g5 A) R
 end.
 
-Definition open_sig_sort_wrt_tm_rec (k:nat) (a5:tm) (sig_sort5:sig_sort) : sig_sort :=
-  match sig_sort5 with
-  | (Cs A) => Cs (open_tm_wrt_tm_rec k a5 A)
-  | (Ax a A R) => Ax (open_tm_wrt_tm_rec k a5 a) (open_tm_wrt_tm_rec k a5 A) R
+Definition open_sort_wrt_co_rec (k:nat) (g5:co) (sort5:sort) : sort :=
+  match sort5 with
+  | (Tm A R) => Tm (open_tm_wrt_co_rec k g5 A) R
+  | (Co phi) => Co (open_constraint_wrt_co_rec k g5 phi)
 end.
 
 Definition open_sort_wrt_tm_rec (k:nat) (a5:tm) (sort5:sort) : sort :=
@@ -241,19 +237,25 @@ Definition open_sort_wrt_tm_rec (k:nat) (a5:tm) (sort5:sort) : sort :=
   | (Co phi) => Co (open_constraint_wrt_tm_rec k a5 phi)
 end.
 
+Definition open_sig_sort_wrt_tm_rec (k:nat) (a5:tm) (sig_sort5:sig_sort) : sig_sort :=
+  match sig_sort5 with
+  | (Cs A) => Cs (open_tm_wrt_tm_rec k a5 A)
+  | (Ax a A R) => Ax (open_tm_wrt_tm_rec k a5 a) (open_tm_wrt_tm_rec k a5 A) R
+end.
+
 Definition open_brs_wrt_co g5 brs_6 := open_brs_wrt_co_rec 0 brs_6 g5.
 
 Definition open_tm_wrt_co g5 a5 := open_tm_wrt_co_rec 0 a5 g5.
 
 Definition open_brs_wrt_tm a5 brs_6 := open_brs_wrt_tm_rec 0 brs_6 a5.
 
-Definition open_sort_wrt_co g5 sort5 := open_sort_wrt_co_rec 0 sort5 g5.
-
 Definition open_sig_sort_wrt_co g5 sig_sort5 := open_sig_sort_wrt_co_rec 0 sig_sort5 g5.
+
+Definition open_sort_wrt_co g5 sort5 := open_sort_wrt_co_rec 0 sort5 g5.
 
 Definition open_co_wrt_co g_5 g__6 := open_co_wrt_co_rec 0 g__6 g_5.
 
-Definition open_sig_sort_wrt_tm a5 sig_sort5 := open_sig_sort_wrt_tm_rec 0 sig_sort5 a5.
+Definition open_sort_wrt_tm a5 sort5 := open_sort_wrt_tm_rec 0 sort5 a5.
 
 Definition open_constraint_wrt_co g5 phi5 := open_constraint_wrt_co_rec 0 phi5 g5.
 
@@ -261,7 +263,7 @@ Definition open_constraint_wrt_tm a5 phi5 := open_constraint_wrt_tm_rec 0 phi5 a
 
 Definition open_co_wrt_tm a5 g_5 := open_co_wrt_tm_rec 0 g_5 a5.
 
-Definition open_sort_wrt_tm a5 sort5 := open_sort_wrt_tm_rec 0 sort5 a5.
+Definition open_sig_sort_wrt_tm a5 sig_sort5 := open_sig_sort_wrt_tm_rec 0 sig_sort5 a5.
 
 Definition open_tm_wrt_tm a5 a_6 := open_tm_wrt_tm_rec 0 a_6 a5.
 
@@ -572,18 +574,6 @@ with fv_co_co_constraint (phi5:constraint) : vars :=
   | (Eq a b A R) => (fv_co_co_tm a) \u (fv_co_co_tm b) \u (fv_co_co_tm A)
 end.
 
-Definition fv_tm_tm_sort (sort5:sort) : vars :=
-  match sort5 with
-  | (Tm A R) => (fv_tm_tm_tm A)
-  | (Co phi) => (fv_tm_tm_constraint phi)
-end.
-
-Definition fv_co_co_sort (sort5:sort) : vars :=
-  match sort5 with
-  | (Tm A R) => (fv_co_co_tm A)
-  | (Co phi) => (fv_co_co_constraint phi)
-end.
-
 Definition fv_tm_tm_sig_sort (sig_sort5:sig_sort) : vars :=
   match sig_sort5 with
   | (Cs A) => (fv_tm_tm_tm A)
@@ -594,6 +584,18 @@ Definition fv_co_co_sig_sort (sig_sort5:sig_sort) : vars :=
   match sig_sort5 with
   | (Cs A) => (fv_co_co_tm A)
   | (Ax a A R) => (fv_co_co_tm a) \u (fv_co_co_tm A)
+end.
+
+Definition fv_tm_tm_sort (sort5:sort) : vars :=
+  match sort5 with
+  | (Tm A R) => (fv_tm_tm_tm A)
+  | (Co phi) => (fv_tm_tm_constraint phi)
+end.
+
+Definition fv_co_co_sort (sort5:sort) : vars :=
+  match sort5 with
+  | (Tm A R) => (fv_co_co_tm A)
+  | (Co phi) => (fv_co_co_constraint phi)
 end.
 
 (** substitutions *)
@@ -717,18 +719,6 @@ with co_subst_co_constraint (g5:co) (c5:covar) (phi5:constraint) {struct phi5} :
   | (Eq a b A R) => Eq (co_subst_co_tm g5 c5 a) (co_subst_co_tm g5 c5 b) (co_subst_co_tm g5 c5 A) R
 end.
 
-Definition tm_subst_tm_sort (a5:tm) (x5:tmvar) (sort5:sort) : sort :=
-  match sort5 with
-  | (Tm A R) => Tm (tm_subst_tm_tm a5 x5 A) R
-  | (Co phi) => Co (tm_subst_tm_constraint a5 x5 phi)
-end.
-
-Definition co_subst_co_sort (g5:co) (c5:covar) (sort5:sort) : sort :=
-  match sort5 with
-  | (Tm A R) => Tm (co_subst_co_tm g5 c5 A) R
-  | (Co phi) => Co (co_subst_co_constraint g5 c5 phi)
-end.
-
 Definition tm_subst_tm_sig_sort (a5:tm) (x5:tmvar) (sig_sort5:sig_sort) : sig_sort :=
   match sig_sort5 with
   | (Cs A) => Cs (tm_subst_tm_tm a5 x5 A)
@@ -739,6 +729,18 @@ Definition co_subst_co_sig_sort (g5:co) (c5:covar) (sig_sort5:sig_sort) : sig_so
   match sig_sort5 with
   | (Cs A) => Cs (co_subst_co_tm g5 c5 A)
   | (Ax a A R) => Ax (co_subst_co_tm g5 c5 a) (co_subst_co_tm g5 c5 A) R
+end.
+
+Definition tm_subst_tm_sort (a5:tm) (x5:tmvar) (sort5:sort) : sort :=
+  match sort5 with
+  | (Tm A R) => Tm (tm_subst_tm_tm a5 x5 A) R
+  | (Co phi) => Co (tm_subst_tm_constraint a5 x5 phi)
+end.
+
+Definition co_subst_co_sort (g5:co) (c5:covar) (sort5:sort) : sort :=
+  match sort5 with
+  | (Tm A R) => Tm (co_subst_co_tm g5 c5 A) R
+  | (Co phi) => Co (co_subst_co_constraint g5 c5 phi)
 end.
 
 
@@ -827,6 +829,13 @@ Definition FixTy : tm :=
 Definition an_toplevel : sig := Fix ~ Ax FixDef FixTy Nom.
 
 Definition toplevel : sig := erase_sig an_toplevel Nom.
+
+Fixpoint ctx_to_rctx (G : context) : role_context :=
+  match G with
+  | nil => nil
+  | (x, (Tm A R)) :: G => (x, R) :: (ctx_to_rctx G)
+  | (c, (Co _)) :: G => ctx_to_rctx G
+  end.
 
 
 
@@ -931,43 +940,53 @@ Inductive consistent : tm -> tm -> Prop :=    (* defn consistent *)
      consistent a b.
 
 (* defns Jerased *)
-Inductive erased_tm : tm -> Prop :=    (* defn erased_tm *)
- | erased_a_Bullet : 
-     erased_tm a_Bullet
- | erased_a_Star : 
-     erased_tm a_Star
- | erased_a_Var : forall (x:tmvar),
-     erased_tm (a_Var_f x)
- | erased_a_Abs : forall (L:vars) (rho:relflag) (R1:role) (a:tm),
-      ( forall x , x \notin  L  -> erased_tm  ( open_tm_wrt_tm a (a_Var_f x) )  )  ->
-     erased_tm  ( (a_UAbs rho R1 a) ) 
- | erased_a_App : forall (a:tm) (rho:relflag) (R1:role) (b:tm),
-     erased_tm a ->
-     erased_tm b ->
-     erased_tm  ( (a_App a rho R1 b) ) 
- | erased_a_Pi : forall (L:vars) (rho:relflag) (A:tm) (R1:role) (B:tm),
-     erased_tm A ->
-      ( forall x , x \notin  L  -> erased_tm  ( open_tm_wrt_tm B (a_Var_f x) )  )  ->
-     erased_tm  ( (a_Pi rho A R1 B) ) 
- | erased_a_CPi : forall (L:vars) (a b A:tm) (R1:role) (B:tm),
-     erased_tm a ->
-     erased_tm b ->
-     erased_tm A ->
-      ( forall c , c \notin  L  -> erased_tm  ( open_tm_wrt_co B (g_Var_f c) )  )  ->
-     erased_tm  ( (a_CPi (Eq a b A R1) B) ) 
- | erased_a_CAbs : forall (L:vars) (b:tm),
-      ( forall c , c \notin  L  -> erased_tm  ( open_tm_wrt_co b (g_Var_f c) )  )  ->
-     erased_tm  ( (a_UCAbs b) ) 
- | erased_a_CApp : forall (a:tm),
-     erased_tm a ->
-     erased_tm  ( (a_CApp a g_Triv) ) 
- | erased_a_Fam : forall (F:tyfam),
-     erased_tm (a_Fam F)
- | erased_a_Const : forall (T:const),
-     erased_tm (a_Const T)
- | erased_a_Conv : forall (a:tm) (R:role),
-     erased_tm a ->
-     erased_tm  ( (a_Conv a R g_Triv) ) .
+Inductive erased_tm : role_context -> tm -> role -> Prop :=    (* defn erased_tm *)
+ | erased_a_Bullet : forall (W:role_context) (R:role),
+      uniq  W  ->
+     erased_tm W a_Bullet R
+ | erased_a_Star : forall (W:role_context) (R:role),
+      uniq  W  ->
+     erased_tm W a_Star R
+ | erased_a_Var : forall (W:role_context) (x:tmvar) (R:role),
+      uniq  W  ->
+      binds  x   R   W  ->
+     erased_tm W (a_Var_f x) R
+ | erased_a_Abs : forall (L:vars) (W:role_context) (rho:relflag) (R1:role) (a:tm) (R:role),
+      ( forall x , x \notin  L  -> erased_tm  (( x  ~  R1 ) ++  W )   ( open_tm_wrt_tm a (a_Var_f x) )  R )  ->
+     erased_tm W  ( (a_UAbs rho R1 a) )  R
+ | erased_a_App : forall (W:role_context) (a:tm) (rho:relflag) (R1:role) (b:tm) (R:role),
+     erased_tm W a R ->
+     erased_tm W b R1 ->
+     erased_tm W  ( (a_App a rho R1 b) )  R
+ | erased_a_Pi : forall (L:vars) (W:role_context) (rho:relflag) (A:tm) (R1:role) (B:tm) (R:role),
+     erased_tm W A R1 ->
+      ( forall x , x \notin  L  -> erased_tm  (( x  ~  R1 ) ++  W )   ( open_tm_wrt_tm B (a_Var_f x) )  R )  ->
+     erased_tm W  ( (a_Pi rho A R1 B) )  R
+ | erased_a_CPi : forall (L:vars) (W:role_context) (a b A:tm) (R1:role) (B:tm) (R:role),
+     erased_tm W a R1 ->
+     erased_tm W b R1 ->
+     erased_tm W A R1 ->
+      ( forall c , c \notin  L  -> erased_tm W  ( open_tm_wrt_co B (g_Var_f c) )  R )  ->
+     erased_tm W  ( (a_CPi (Eq a b A R1) B) )  R
+ | erased_a_CAbs : forall (L:vars) (W:role_context) (b:tm) (R:role),
+      ( forall c , c \notin  L  -> erased_tm W  ( open_tm_wrt_co b (g_Var_f c) )  R )  ->
+     erased_tm W  ( (a_UCAbs b) )  R
+ | erased_a_CApp : forall (W:role_context) (a:tm) (R:role),
+     erased_tm W a R ->
+     erased_tm W  ( (a_CApp a g_Triv) )  R
+ | erased_a_Fam : forall (W:role_context) (F:tyfam) (R:role),
+      uniq  W  ->
+     erased_tm W (a_Fam F) R
+ | erased_a_Const : forall (W:role_context) (T:const) (R:role),
+      uniq  W  ->
+     erased_tm W (a_Const T) R
+ | erased_a_Conv : forall (W:role_context) (a:tm) (R1 R:role),
+     erased_tm W a R ->
+     erased_tm W  ( (a_Conv a R1 g_Triv) )  R
+ | erased_a_Sub : forall (W:role_context) (a:tm) (R2 R1:role),
+     erased_tm W a R1 ->
+     SubRole R1 R2 ->
+     erased_tm W a R2.
 
 (* defns JChk *)
 Inductive RhoCheck : relflag -> tmvar -> tm -> Prop :=    (* defn RhoCheck *)
@@ -979,75 +998,71 @@ Inductive RhoCheck : relflag -> tmvar -> tm -> Prop :=    (* defn RhoCheck *)
      RhoCheck Irrel x A.
 
 (* defns Jpar *)
-Inductive Par : context -> available_props -> tm -> tm -> role -> Prop :=    (* defn Par *)
- | Par_Refl : forall (G:context) (D:available_props) (a:tm) (R:role),
+Inductive Par : context -> available_props -> role_context -> tm -> tm -> role -> Prop :=    (* defn Par *)
+ | Par_Refl : forall (G:context) (D:available_props) (W:role_context) (a:tm) (R:role),
+     erased_tm W a R ->
+     Par G D W a a R
+ | Par_Beta : forall (G:context) (D:available_props) (W:role_context) (a:tm) (rho:relflag) (R1:role) (b a' b':tm) (R:role),
+     Par G D W a  ( (a_UAbs rho R1 a') )  R ->
+     Par G D W b b' R1 ->
+     Par G D W (a_App a rho R1 b)  (open_tm_wrt_tm  a'   b' )  R
+ | Par_App : forall (G:context) (D:available_props) (W:role_context) (a:tm) (rho:relflag) (R1:role) (b a' b':tm) (R:role),
+     Par G D W a a' R ->
+     Par G D W b b' R1 ->
+     Par G D W (a_App a rho R1 b) (a_App a' rho R1 b') R
+ | Par_CBeta : forall (G:context) (D:available_props) (W:role_context) (a a':tm) (R:role),
+     Par G D W a  ( (a_UCAbs a') )  R ->
+     Par G D W (a_CApp a g_Triv)  (open_tm_wrt_co  a'   g_Triv )  R
+ | Par_CApp : forall (G:context) (D:available_props) (W:role_context) (a a':tm) (R:role),
+     Par G D W a a' R ->
+     Par G D W (a_CApp a g_Triv) (a_CApp a' g_Triv) R
+ | Par_Abs : forall (L:vars) (G:context) (D:available_props) (W:role_context) (rho:relflag) (R1:role) (a a':tm) (R:role),
+      ( forall x , x \notin  L  -> Par G D  (( x  ~  R1 ) ++  W )   ( open_tm_wrt_tm a (a_Var_f x) )   ( open_tm_wrt_tm a' (a_Var_f x) )  R )  ->
+     Par G D W (a_UAbs rho R1 a) (a_UAbs rho R1 a') R
+ | Par_Pi : forall (L:vars) (G:context) (D:available_props) (W:role_context) (rho:relflag) (A:tm) (R1:role) (B A' B':tm) (R:role),
+     Par G D W A A' R1 ->
+      ( forall x , x \notin  L  -> Par G D  (( x  ~  R1 ) ++  W )   ( open_tm_wrt_tm B (a_Var_f x) )   ( open_tm_wrt_tm B' (a_Var_f x) )  R )  ->
+     Par G D W (a_Pi rho A R1 B) (a_Pi rho A' R1 B') R
+ | Par_CAbs : forall (L:vars) (G:context) (D:available_props) (W:role_context) (a a':tm) (R:role),
+      ( forall c , c \notin  L  -> Par G D W  ( open_tm_wrt_co a (g_Var_f c) )   ( open_tm_wrt_co a' (g_Var_f c) )  R )  ->
+     Par G D W (a_UCAbs a) (a_UCAbs a') R
+ | Par_CPi : forall (L:vars) (G:context) (D:available_props) (W:role_context) (a b A:tm) (R1:role) (B a' b' A' B':tm) (R:role),
+     Par G D W A A' R1 ->
+     Par G D W a a' R1 ->
+     Par G D W b b' R1 ->
+      ( forall c , c \notin  L  -> Par G D W  ( open_tm_wrt_co B (g_Var_f c) )   ( open_tm_wrt_co B' (g_Var_f c) )  R )  ->
+     Par G D W (a_CPi (Eq a b A R1) B) (a_CPi (Eq a' b' A' R1) B') R
+ | Par_Axiom : forall (G:context) (D:available_props) (W:role_context) (F:tyfam) (a:tm) (R:role) (A:tm) (R1:role),
+      binds  F  (Ax  a A R1 )   toplevel   ->
+     SubRole R1 R ->
+      uniq  W  ->
+     Par G D W (a_Fam F) a R
+ | Par_Cong : forall (G:context) (D:available_props) (W:role_context) (a1:tm) (R:role) (a2:tm) (R1:role),
+     Par G D W a1 a2 R1 ->
+     Par G D W (a_Conv a1 R g_Triv) (a_Conv a2 R g_Triv) R1
+ | Par_Combine : forall (G:context) (D:available_props) (W:role_context) (a1:tm) (R:role) (a2:tm) (R1:role),
+     Par G D W a1  ( (a_Conv a2 R g_Triv) )  R1 ->
+     Par G D W  ( (a_Conv a1 R g_Triv) )   ( (a_Conv a2 R g_Triv) )  R1
+ | Par_Push : forall (G:context) (D:available_props) (W:role_context) (a1:tm) (R2:role) (b1 a2 b2:tm) (R R1:role),
+     Par G D W a1  ( (a_Conv a2 R g_Triv) )  R1 ->
+     Par G D W b1 b2 R2 ->
+     Par G D W  (a_App  a1  Rel  R2   b1 )  (a_Conv  (  (a_App  a2  Rel  R2    ( (a_Conv b2 R g_Triv) )  )  )  R g_Triv) R1
+ | Par_CPush : forall (G:context) (D:available_props) (W:role_context) (a1 a2:tm) (R R1:role),
+     Par G D W a1  ( (a_Conv a2 R g_Triv) )  R1 ->
+     Par G D W (a_CApp a1 g_Triv) (a_Conv  ( (a_CApp a2 g_Triv) )  R g_Triv) R1
+with MultiPar : context -> available_props -> role_context -> tm -> tm -> role -> Prop :=    (* defn MultiPar *)
+ | MP_Refl : forall (G:context) (D:available_props) (W:role_context) (a:tm) (R:role),
      lc_tm a ->
-     Par G D a a R
- | Par_Beta : forall (G:context) (D:available_props) (a:tm) (rho:relflag) (R:role) (b a' b':tm) (R1:role),
-     Par G D a  ( (a_UAbs rho R a') )  R1 ->
-     Par G D b b' R ->
-     SubRole R R1 ->
-     Par G D (a_App a rho R b)  (open_tm_wrt_tm  a'   b' )  R1
- | Par_App : forall (G:context) (D:available_props) (a:tm) (rho:relflag) (R:role) (b a' b':tm) (R1:role),
-     Par G D a a' R1 ->
-     Par G D b b' R ->
-     SubRole R R1 ->
-     Par G D (a_App a rho R b) (a_App a' rho R b') R1
- | Par_CBeta : forall (G:context) (D:available_props) (a a':tm) (R:role),
-     Par G D a  ( (a_UCAbs a') )  R ->
-     Par G D (a_CApp a g_Triv)  (open_tm_wrt_co  a'   g_Triv )  R
- | Par_CApp : forall (G:context) (D:available_props) (a a':tm) (R:role),
-     Par G D a a' R ->
-     Par G D (a_CApp a g_Triv) (a_CApp a' g_Triv) R
- | Par_Abs : forall (L:vars) (G:context) (D:available_props) (rho:relflag) (R:role) (a a':tm) (R1:role),
-      ( forall x , x \notin  L  -> Par G D  ( open_tm_wrt_tm a (a_Var_f x) )   ( open_tm_wrt_tm a' (a_Var_f x) )  R1 )  ->
-     Par G D (a_UAbs rho R a) (a_UAbs rho R a') R1
- | Par_Pi : forall (L:vars) (G:context) (D:available_props) (rho:relflag) (A:tm) (R:role) (B A' B':tm) (R1:role),
-     Par G D A A' R ->
-      ( forall x , x \notin  L  -> Par G D  ( open_tm_wrt_tm B (a_Var_f x) )   ( open_tm_wrt_tm B' (a_Var_f x) )  R1 )  ->
-     SubRole R R1 ->
-     Par G D (a_Pi rho A R B) (a_Pi rho A' R B') R1
- | Par_CAbs : forall (L:vars) (G:context) (D:available_props) (a a':tm) (R:role),
-      ( forall c , c \notin  L  -> Par G D  ( open_tm_wrt_co a (g_Var_f c) )   ( open_tm_wrt_co a' (g_Var_f c) )  R )  ->
-     Par G D (a_UCAbs a) (a_UCAbs a') R
- | Par_CPi : forall (L:vars) (G:context) (D:available_props) (A B A1:tm) (R:role) (a A' B' A1' a':tm) (R1:role),
-     Par G D A A' R ->
-     Par G D B B' R ->
-      ( forall c , c \notin  L  -> Par G D  ( open_tm_wrt_co a (g_Var_f c) )   ( open_tm_wrt_co a' (g_Var_f c) )  R1 )  ->
-     Par G D A1 A1' R ->
-     SubRole R R1 ->
-     Par G D (a_CPi (Eq A B A1 R) a) (a_CPi (Eq A' B' A1' R) a') R1
- | Par_Axiom : forall (G:context) (D:available_props) (F:tyfam) (a:tm) (R1:role) (A:tm) (R:role),
-      binds  F  (Ax  a A R )   toplevel   ->
-     SubRole R R1 ->
-     Par G D (a_Fam F) a R1
- | Par_Cong : forall (G:context) (D:available_props) (a1:tm) (R:role) (a2:tm) (R1:role),
-     Par G D a1 a2 R1 ->
-     Par G D (a_Conv a1 R g_Triv) (a_Conv a2 R g_Triv) R1
- | Par_Combine : forall (G:context) (D:available_props) (a1:tm) (R:role) (a2:tm) (R1:role),
-     Par G D a1  ( (a_Conv a2 R g_Triv) )  R1 ->
-     Par G D  ( (a_Conv a1 R g_Triv) )   ( (a_Conv a2 R g_Triv) )  R1
- | Par_Push : forall (G:context) (D:available_props) (a1:tm) (R2:role) (b1 a2 b2:tm) (R R1:role),
-     Par G D a1  ( (a_Conv a2 R g_Triv) )  R1 ->
-     Par G D b1 b2 R2 ->
-     SubRole R2 R1 ->
-     Par G D  (a_App  a1  Rel  R2   b1 )  (a_Conv  (  (a_App  a2  Rel  R2    ( (a_Conv b2 R g_Triv) )  )  )  R g_Triv) R1
- | Par_CPush : forall (G:context) (D:available_props) (a1 a2:tm) (R R1:role),
-     Par G D a1  ( (a_Conv a2 R g_Triv) )  R1 ->
-     Par G D (a_CApp a1 g_Triv) (a_Conv  ( (a_CApp a2 g_Triv) )  R g_Triv) R1
-with MultiPar : context -> available_props -> tm -> tm -> role -> Prop :=    (* defn MultiPar *)
- | MP_Refl : forall (G:context) (D:available_props) (a:tm) (R:role),
-     lc_tm a ->
-     MultiPar G D a a R
- | MP_Step : forall (G:context) (D:available_props) (a a':tm) (R:role) (b:tm),
-     Par G D a b R ->
-     MultiPar G D b a' R ->
-     MultiPar G D a a' R
-with joins : context -> available_props -> tm -> tm -> role -> Prop :=    (* defn joins *)
- | join : forall (G:context) (D:available_props) (a1 a2:tm) (R:role) (b:tm),
-     MultiPar G D a1 b R ->
-     MultiPar G D a2 b R ->
-     joins G D a1 a2 R.
+     MultiPar G D W a a R
+ | MP_Step : forall (G:context) (D:available_props) (W:role_context) (a a':tm) (R:role) (b:tm),
+     Par G D W a b R ->
+     MultiPar G D W b a' R ->
+     MultiPar G D W a a' R
+with joins : context -> available_props -> role_context -> tm -> tm -> role -> Prop :=    (* defn joins *)
+ | join : forall (G:context) (D:available_props) (W:role_context) (a1 a2:tm) (R:role) (b:tm),
+     MultiPar G D W a1 b R ->
+     MultiPar G D W a2 b R ->
+     joins G D W a1 a2 R.
 
 (* defns Jbeta *)
 Inductive Beta : tm -> tm -> role -> Prop :=    (* defn Beta *)
